LambdaLetDollar.v
@@ -142,7 +142,7 @@ Proof.
 Qed.
 
 
-Fixpoint map' {A B : Type} (f : A -> B) (e : tm' A) : tm' B :=
+Fixpoint map' {A B : Type} (f : A → B) (e : tm' A) : tm' B :=
   match e with
   | <| var a |> => <| var {f a} |>
   | <| S₀ |> => <| S₀ |>
@@ -158,7 +158,7 @@ Definition mapV' {A B} (f : A → B) (v : val' A) : val' B :=
   | val_s_0' => val_s_0'
   end.
 
-Definition mapP' {A B : Type} (f : A -> B) (p : non' A) : non' B :=
+Definition mapP' {A B : Type} (f : A → B) (p : non' A) : non' B :=
   match p with
   | non_app' e1 e2 => non_app' (map' f e1) (map' f e2)
   | non_dol' e1 e2 => non_dol' (map' f e1) (map' f e2)
@@ -194,7 +194,14 @@ Proof.
   intros. destruct p; auto.
 Qed.
 
-Lemma map_map_law' : forall A e B C (f:A->B) (g:B->C),
+Lemma map_id_law' : ∀ A (e : tm' A),
+  map' id e = e.
+Proof.
+  induction e; cbn; auto;
+  repeat rewrite option_map_id_law; f_equal; auto.
+Qed.
+
+Lemma map_map_law' : ∀ A e B C (f : A → B) (g : B → C),
   map' g (map' f e) = map' (g ∘ f) e.
 Proof.
   intros. generalize dependent B. generalize dependent C.
@@ -205,7 +212,7 @@ Proof.
   rewrite option_map_comp_law; auto.
 Qed.
 
-Lemma mapV_mapV_law' : forall A v B C (f : A → B) (g : B → C),
+Lemma mapV_mapV_law' : ∀ A v B C (f : A → B) (g : B → C),
   mapV' g (mapV' f v) = mapV' (g ∘ f) v.
 Proof.
   destruct v; intros; cbn; auto.
@@ -213,7 +220,7 @@ Proof.
   rewrite option_map_comp_law. reflexivity.
 Qed.
 
-Fixpoint bind' {A B : Type} (f : A -> tm' B) (e : tm' A) : tm' B :=
+Fixpoint bind' {A B : Type} (f : A → tm' B) (e : tm' A) : tm' B :=
   match e with
   | <| var a |> => f a
   | <| S₀ |> => <| S₀ |>
@@ -241,7 +248,7 @@ Definition bindV' {A B} (f : A → tm' B) (v : val' A) : val' B :=
       end) e)
   end.
 
-Definition bindP' {A B : Type} (f : A -> tm' B) (p : non' A) : non' B :=
+Definition bindP' {A B : Type} (f : A → tm' B) (p : non' A) : non' B :=
   match p with
   | non_app' e1 e2 => non_app' (bind' f e1) (bind' f e2)
   | non_dol' e1 e2 => non_dol' (bind' f e1) (bind' f e2)
@@ -631,7 +638,7 @@ Definition mapJ' {A B} (f : A → B) (j : J' A) : J' B :=
   | J_dol' e => J_dol' (map' f e)
   end.
 
-Lemma mapJ_mapJ_law' : forall A j B C (f : A → B) (g : B → C),
+Lemma mapJ_mapJ_law' : ∀ A j B C (f : A → B) (g : B → C),
   mapJ' g (mapJ' f j) = mapJ' (g ∘ f) j.
 Proof.
   destruct j; intros; cbn;
@@ -646,7 +653,7 @@ Fixpoint mapK' {A B} (f : A → B) (k : K' A) : K' B :=
   | K_let' k1 e2 => K_let' (mapK' f k1) (map' (option_map f) e2)
   end.
 
-Lemma mapK_mapK_law' : forall A k B C (f : A → B) (g : B → C),
+Lemma mapK_mapK_law' : ∀ A k B C (f : A → B) (g : B → C),
   mapK' g (mapK' f k) = mapK' (g ∘ f) k.
 Proof.
   induction k; intros; cbn; auto.
